The very first phase-2 low-level impl. of the Merkle tree

secure_api/merkle_tree/MerkleTree.New.Low.fst
@@ -51,15 +51,18 @@ assume val hash_2:
 // A Merkle tree `MT i j hs` stores all necessary hashes to generate
 // a Merkle path for each element from the index `i` to `j-1`. 
 // `hs` is a 2-dim store for hashes, where `hs[0]` contains leaf hash values.
+// `ths` is a store for "rightmost" hashes, manipulated only when required to
+// calculate some merkle paths that need the rightmost hashes as a part of them.
 noeq type merkle_tree = 
 | MT: i:uint32_t -> j:uint32_t{j > i} ->
-      hs:B.buffer hash_vec{B.length hs = U32.n} ->
+      hs:B.buffer hash_vec{B.length hs = 32} ->
+      ths:hash_vec{V.size_of ths = 32ul} ->
       merkle_tree
 
 /// Construction
 
 val create_mt_: 
-  hs:B.buffer hash_vec{B.length hs = U32.n} ->
+  hs:B.buffer hash_vec{B.length hs = 32} ->
   depth:uint32_t{depth <= 32ul} ->
   HST.ST unit
 	 (requires (fun h0 -> 
@@ -82,20 +85,21 @@ let create_mt _ =
   let mt_region = BV.new_region_ HH.root in
   let hs = B.malloc mt_region (BV.create_empty uint8_t) 32ul in
   create_mt_ hs 32ul;
-  MT 0ul 1ul hs
+  let ths = BV.create 0uy hash_size 32ul in
+  MT 0ul 1ul hs ths
 
 /// Destruction (free)
 
 val free_mt_:
   lv:uint32_t{lv <= 32ul} ->
-  hs:B.buffer hash_vec{B.length hs = U32.n} ->
+  hs:B.buffer hash_vec{B.length hs = 32} ->
   HST.ST unit
 	 (requires (fun h0 -> true))
 	 (ensures (fun h0 _ h1 -> true))
 let rec free_mt_ lv hs =
   admit ();
   if lv = 0ul then ()
-  else (V.free (B.index hs (lv - 1ul));
+  else (BV.free hash_size (B.index hs (lv - 1ul));
        free_mt_ (lv - 1ul) hs)
 
 val free_mt: merkle_tree ->
@@ -105,6 +109,7 @@ val free_mt: merkle_tree ->
 let free_mt mt =
   admit ();
   free_mt_ 32ul (MT?.hs mt);
+  BV.free hash_size (MT?.ths mt);
   B.free (MT?.hs mt)
 
 /// Insertion
@@ -112,7 +117,7 @@ let free_mt mt =
 val insert_:
   lv:uint32_t{lv < 32ul} ->
   j:uint32_t ->
-  hs:B.buffer hash_vec{B.length hs = U32.n} ->
+  hs:B.buffer hash_vec{B.length hs = 32} ->
   acc:hash ->
   HST.ST unit
 	 (requires (fun h0 -> true))
@@ -139,38 +144,70 @@ let rec insert mt v =
   MT (MT?.i mt)
      (MT?.j mt + 1ul)
      (MT?.hs mt)
+     (MT?.ths mt)
 
 /// Getting the Merkle root and path
 
-val mt_get_path_:
-  hs:B.buffer hash_vec{B.length hs = U32.n} ->
+val fill_rightmost:
   lv:uint32_t{lv < 32ul} ->
-  i:uint32_t -> j:uint32_t ->
-  k:uint32_t{i <= k && k < j} ->
-  path:B.buffer hash{B.length path = U32.n} ->
-  acc:hash ->
+  hs:B.buffer hash_vec{B.length hs = 32} ->
+  ths:hash_vec{V.size_of ths = 32ul} ->
+  j:uint32_t ->
+  acc:hash -> actd:bool ->
   HST.ST unit
 	 (requires (fun h0 -> true))
 	 (ensures (fun h0 _ h1 -> true))
-let rec mt_get_path_ hs lv i j k path acc =
-  admit ()
+let rec fill_rightmost lv hs ths j acc actd =
+  admit ();
+  if j = 0ul then ()
+  else if j % 2ul = 0ul
+  then fill_rightmost (lv + 1ul) hs ths (j / 2ul) acc actd
+  else (
+    (if actd
+    then (hash_2 (V.index (B.index hs lv) (j - 1ul)) acc acc;
+	 BV.assign_copy hash_size ths (lv + 1ul) acc)
+    else B.blit (V.index (B.index hs lv) (j - 1ul)) 0ul acc 0ul hash_size);
+    fill_rightmost (lv + 1ul) hs ths (j / 2ul) acc true)
+
+// Assuming the rightmost hashes (`ths`) are already calculated
+val mt_get_path_:
+  lv:uint32_t{lv < 32ul} ->
+  hs:B.buffer hash_vec{B.length hs = 32} ->
+  ths:hash_vec{V.size_of ths = 32ul} ->
+  j:uint32_t -> k:uint32_t{j = 0ul || k < j} ->
+  path:B.buffer hash{B.length path = 32} ->
+  HST.ST unit
+	 (requires (fun h0 -> true))
+	 (ensures (fun h0 _ h1 -> true))
+let rec mt_get_path_ lv hs ths j k path =
+  admit ();
+  if j = 0ul then ()
+  else if k % 2ul = 0ul 
+  then (if k + 1ul < j
+       then (B.upd path lv (V.index (B.index hs lv) (k + 1ul));
+	    mt_get_path_ (lv + 1ul) hs ths (j / 2ul) (k / 2ul) path)
+       else (B.upd path lv (V.index ths lv);
+	    mt_get_path_ (lv + 1ul) hs ths (j / 2ul) (k / 2ul) path))
+  else (B.upd path lv (V.index (B.index hs lv) (k - 1ul));
+       mt_get_path_ (lv + 1ul) hs ths (j / 2ul) (k / 2ul) path)
 
 val mt_get_path:
   mt:merkle_tree -> 
   idx:uint32_t{MT?.i mt <= idx && idx < MT?.j mt} ->
   root:hash ->
-  path:B.buffer hash{B.length path = U32.n} ->
+  path:B.buffer hash{B.length path = 32} ->
   HST.ST uint32_t
 	 (requires (fun h0 -> true))
 	 (ensures (fun h0 _ h1 -> true))
 let mt_get_path mt idx root path =
-  mt_get_path_ (MT?.hs mt) 0ul (MT?.i mt) (MT?.j mt) idx path root;
+  fill_rightmost 0ul (MT?.hs mt) (MT?.ths mt) (MT?.j mt) root false;
+  mt_get_path_ 0ul (MT?.hs mt) (MT?.ths mt) (MT?.j mt) idx path;
   MT?.j mt
 
 /// Flushing
 
-// TODO: need to think about flushing after deciding a proper data structure
-//       for `MT?.hs`.
+// TODO: need to think about flushing after deciding a proper 
+//       data structure for `MT?.hs`.
 // NOTE: flush "until" `idx`
 val mt_flush_to:
   mt:merkle_tree ->
@@ -194,7 +231,7 @@ val mt_verify_:
   lv:uint32_t{lv < 32ul} ->
   k:uint32_t ->
   j:uint32_t{j = 0ul || k < j} ->
-  path:B.buffer hash{B.length path = U32.n} ->
+  path:B.buffer hash{B.length path = 32} ->
   acc:hash ->
   HST.ST unit
 	 (requires (fun h0 -> true))
@@ -209,4 +246,33 @@ let rec mt_verify_ lv k j path acc =
 	 else ())
     else hash_2 (B.index path lv) acc acc;
     mt_verify_ (lv + 1ul) (k / 2ul) (j / 2ul) path acc)
+
+val buf_eq:
+  #a:eqtype -> b1:B.buffer a -> b2:B.buffer a ->
+  len:uint32_t ->
+  HST.ST bool
+	 (requires (fun h0 -> 
+	   B.live h0 b1 /\ B.live h0 b2 /\
+	   len <= B.len b1 /\ len <= B.len b2))
+	 (ensures (fun h0 _ h1 -> true))
+let rec buf_eq #a b1 b2 len =
+  if len = 0ul then true
+  else (let a1 = B.index b1 (len - 1ul) in
+       let a2 = B.index b2 (len - 1ul) in
+       let teq = buf_eq b1 b2 (len - 1ul) in
+       a1 = a2 && teq)
+
+val mt_verify:
+  k:uint32_t ->
+  j:uint32_t{k < j} ->
+  path:B.buffer hash{B.length path = 32} ->
+  root:hash ->
+  HST.ST bool
+	 (requires (fun h0 -> true))
+	 (ensures (fun h0 _ h1 -> true))
+let mt_verify k j path root =
+  admit ();
+  let acc = B.malloc HH.root 0uy hash_size in
+  mt_verify_ 0ul k j path acc;
+  buf_eq acc root hash_size
 
